theories/Proofs.v
@@ -1,7 +1,9 @@
 (** * Proofs: definition of free-variable tableaux proofs. *)
 
 From Stdlib Require Import Classical.
+From Stdlib Require Import Lia.
 
+From Tableaux Require Import Choice.
 From Tableaux Require Import Semantics.
 From Tableaux Require Import Skolemization.
 From Tableaux Require Import Syntax.
@@ -234,6 +236,7 @@ Section TableauxProofs.
 End TableauxProofs.
 Arguments is_tableau_satisfiable {_ _ _ _ _} _ _ {_ _ _} _.
 
+(** ** Some usual properties of tableaux *)
 Section TableauxProperties.
   Context `{set_nat : set nat} {pred func var : Atom} (sko : Skolemization_ pred func var).
 
@@ -288,6 +291,236 @@ Section TableauxProperties.
   Qed.
 End TableauxProperties.
 
+(** ** Tableaux using expansion *)
+
+(** In this section, we develop the expansion of tableaux. Instead of defining them as inductive
+    trees, we define trees with sequence of expansions corresponding to the rules defined in
+    [hasTableau_]. Then, we can show that having a closed sequence of tableaux expansion is
+    the same as having an [hasTableau_]. Moreover, the satisfiability of a sequence of tableaux
+    is equivalent to the satisfiability of an [hasTableau_], which allow to show e.g. soundness
+    of the [hasTableau_] inductive. *)
+
+Reserved Notation "T |> T'" (at level 99, right associativity).
+Section TableauxExpansion.
+  Context `{set_nat : set nat} {pred func var : Atom} (sko : Skolemization_ pred func var).
+
+  Let Con := Con_ pred func var.
+  Let Form := Form_ pred func var.
+  Let Term := Term_ func var.
+
+  (** *** [ExpansionTableau] *)
+  Section Def.
+    (** We define an [ExpansionTableau] as a simple list of contexts. *)
+    (* TODO: add a [sko_record] in the definition. *)
+    Definition ExpansionTableau := list Con.
+
+    (** Make an [ExpansionTableau] from a single [Con]. *)
+    Definition mkExpansionTableau (Gamma : Con) : ExpansionTableau := [Gamma].
+
+    (** Then, a [Branch] is simply a [Con]. *)
+    Definition Branch := Con.
+
+    (** We say that [B] is the [nth_branch_of T] if [T.(i)] is [B]. *)
+    Definition nth_branch_of (T : ExpansionTableau) (i : nat) : option Branch := T.(i).
+
+    (** A branch [B] contains [F] is [F \in B]. *)
+    Definition branch_contains (B : Branch) (F : Form) : Prop := F \in B.
+
+    (** To add [F] in a branch [B] in an [ExpansionTableau] [T], it suffices to replace
+        [B] by by [F :: B]. *)
+    Definition add_in_branch
+      (T : ExpansionTableau) (i : nat) (F : Form) : ExpansionTableau :=
+      match nth_branch_of T i with
+      | None => T
+      | Some B => replace_nth i (B ,, F) T
+      end.
+
+    Definition add_branch (T : ExpansionTableau) (F : Form) (B : Branch) : ExpansionTableau :=
+      (B ,, F) :: T.
+
+    Definition branch_to_con (B : Branch) : Con := B.
+
+    (** An [ExpansionTableau] is said [satisfiable] if one of its branches is satisfiable. *)
+    Definition is_satisfiable_ExpansionTableau (T : ExpansionTableau) : Prop :=
+      exists (M : Model pred func), forall (mu : env M var),
+        exists (B : Branch), List.In B T /\ [[ M # [] # mu '|= ctx_to_form (branch_to_con B) ]].
+
+    (** An [ExpansionTableau] is said [closed] if there exists a substitution [sigma] such that
+        every branch of [T] has a contradiction. *)
+    Definition is_closed_ExpansionTableau (T : ExpansionTableau) :=
+      exists (sigma : Substitution var Term),
+        List.Forall
+          (fun B => branch_contains B Bot \/
+                   exists (P P' : Form),
+                     branch_contains B P /\ branch_contains B (Neg P') /\
+                       (Neg P')@[sigma] = P@[sigma]) T.
+
+    (** If a context is satisfiable, then so is its associated [ExpansionTableau]. *)
+    Lemma ctx_satisfiable_ExpansionTableau_satisfiable :
+      forall (Gamma : Con),
+        is_satisfiable (ctx_to_form Gamma) ->
+        is_satisfiable_ExpansionTableau (mkExpansionTableau Gamma).
+    Proof using Type.
+      intros ? (M & hinterp). exists M; intro mu; exists Gamma; split.
+      - now left.
+      - apply hinterp.
+    Qed.
+
+    Lemma is_satisfiable_is_satisfiable_add_in_branch :
+      forall (T : ExpansionTableau) (B : Branch) (F G : Form) (i : nat),
+        nth_branch_of T i = Some B ->
+        is_satisfiable_ExpansionTableau T -> branch_contains B F -> imply F G ->
+        is_satisfiable_ExpansionTableau (add_in_branch T i G).
+    Proof using Type.
+      intros ????? ei (M & hsat) hcontains himp. exists M; intro mu. specialize (hsat mu).
+      destruct hsat as (B0 & hin & hinterp). apply In_nth_error in hin; destruct hin as (j & ej).
+      destruct (i == j); subst.
+      - unfold nth_branch_of in ei; rewrite ei in ej; injection ej => eB; clear ej; subst.
+        exists (B0 ,, G); split.
+        + unfold add_in_branch, nth_branch_of. rewrite ei.
+          eapply In_replace_nth; eauto.
+        + eapply extend_with_imply_form; eauto.
+      - exists B0; split; auto.
+        unfold add_in_branch; rewrite ei. eapply In_replace_nth'; eauto.
+    Qed.
+
+    Lemma is_satisfiable_is_satisfiable_or :
+      forall (T : ExpansionTableau) (B : Branch) (F G : Form) (i : nat),
+        nth_branch_of T i = Some B -> branch_contains B (Or F G) ->
+        is_satisfiable_ExpansionTableau T ->
+        is_satisfiable_ExpansionTableau (add_branch (add_in_branch T i F) G B).
+    Proof using Type.
+      intros ????? ei hcontains (M & hsat). exists M; intro mu. specialize (hsat mu).
+      destruct hsat as (B0 & hin & hinterp). apply In_nth_error in hin; destruct hin as (j & ej).
+      destruct (i == j); subst.
+      - unfold nth_branch_of in ei; rewrite ei in ej; injection ej => eB; clear ej; subst.
+        have hinterpOr := in_form_list_interp hcontains hinterp.
+        cbn in hinterpOr. destruct hinterpOr as [hF | hG].
+        + exists (B0 ,, F); split.
+          * right. unfold add_in_branch, nth_branch_of. rewrite ei.
+            eapply In_replace_nth; eauto.
+          * cbn; intros [hnF | hnB0]; auto.
+        + exists (B0 ,, G); split.
+          * now left.
+          * cbn; intros [hnG | hnB0]; auto.
+      - exists B0; split; auto. right. unfold add_in_branch. rewrite ei.
+        eapply In_replace_nth'; eauto.
+    Qed.
+
+    Lemma add_in_branch_get :
+      forall (T : ExpansionTableau) (B : Branch) (i : nat) (F : Form),
+        nth_branch_of T i = Some B ->
+        nth_branch_of (add_in_branch T i F) i = Some (B ,, F).
+    Proof using Type.
+      intros ???? e; unfold nth_branch_of in e |- *.
+      unfold add_in_branch, nth_branch_of; rewrite e.
+      erewrite get_replace_nth; eauto.
+    Qed.
+
+    Lemma branch_contains_add :
+      forall (B : Branch) (F G : Form),
+        branch_contains B F -> branch_contains (B ,, G) F.
+    Proof using Type. intros. now right. Qed.
+  End Def.
+  (* We make these opaque as we provide everything needed in the API. *)
+  #[global] Opaque ExpansionTableau.
+  #[global] Opaque Branch.
+
+  (** *** Expansion Sequence *)
+
+  (** We give a relation between [ExpansionTableau] that mirrors the rules of
+      [hasTableau_] *)
+  Inductive ExpansionStep : ExpansionTableau -> ExpansionTableau -> Prop :=
+  | expansion_NegNeg :
+    forall (T : ExpansionTableau) (B : Branch) (F : Form) (i : nat),
+      nth_branch_of T i = Some B -> branch_contains B (Neg (Neg F)) ->
+      T |> (add_in_branch T i F)
+  | expansion_NegOr :
+    forall (T : ExpansionTableau) (B : Branch) (F1 F2 : Form) (i : nat),
+      nth_branch_of T i = Some B -> branch_contains B (Neg (Or F1 F2)) ->
+      T |> (add_in_branch (add_in_branch T i (Neg F1)) i (Neg F2))
+  | expansion_Or :
+    forall (T : ExpansionTableau) (B : Branch) (F1 F2 : Form) (i : nat),
+      nth_branch_of T i = Some B -> branch_contains B (Or F1 F2) ->
+      T |> (add_branch (add_in_branch T i F1) F2 B)
+  | expansion_All :
+    forall (T : ExpansionTableau) (B : Branch) (F : Form) (i : nat) (x : var),
+      nth_branch_of T i = Some B -> branch_contains B (All F) ->
+      T |> (add_in_branch T i (F {0 \to Free x}))
+  | expansion_NegAll :
+    forall (T : ExpansionTableau) (B : Branch) (F : Form) (i : nat) (t : Term)
+      (symbs : sko_record sko),
+      sko t (Neg (All F)) symbs (branch_to_con B) = true ->
+      nth_branch_of T i = Some B -> branch_contains B (Neg (All F)) ->
+      T |> (add_in_branch T i (Neg F {0 \to t}))
+  where "T |> T'" := (ExpansionStep T T').
+
+  (** An [ExpansionSequence] is a list of [ExpansionTableau] where each element is related
+      to another w.r.t. [ExpansionStep]. *)
+  Record ExpansionSequence :=
+    { seq :> list ExpansionTableau
+    ; isSequence :
+      forall (i : nat) (T T' : ExpansionTableau),
+        nth_error seq i = Some T -> nth_error seq (S i) = Some T' -> T |> T' }.
+
+  (** An [ExpansionSequence] that has its first tableau satisfiable has all its
+      [ExpansionTableaux] satisfiable. *)
+  Lemma satisfiable_ExpansionSequence :
+    forall (seq : ExpansionSequence) (T : ExpansionTableau),
+      hd_error seq = Some T -> is_satisfiable_ExpansionTableau T ->
+      forall (i : nat) (T' : ExpansionTableau), nth_error seq i = Some T' ->
+                                         is_satisfiable_ExpansionTableau T'.
+  Proof.
+    intros (seq & hisSeq) T e hsat i; cbn in *. induction i as [|j IHj]; intros T' e'.
+    - rewrite nth_error_0 e in e'. injection e' => <- //.
+    - have h : exists (T0 : ExpansionTableau), seq.(j) = Some T0.
+      { have hlt := nth_error_Some' _ _ _ e'.
+        exists (nth j seq T). apply nth_error_nth'. lia. }
+      destruct h as (T0 & eT0); specialize (IHj T0 eT0).
+      specialize (hisSeq j T0 T' eT0 e'). destruct hisSeq.
+
+      (* Case: [Neg (Neg F)] *)
+      + eapply is_satisfiable_is_satisfiable_add_in_branch; eauto.
+        apply equiv_imply. symmetry; apply neg_neg_equiv.
+
+      (* Case: [Neg (Or F1 F2)] *)
+      + eapply is_satisfiable_is_satisfiable_add_in_branch with
+          (F := Neg (Or F1 F2)) (T := add_in_branch T0 i (Neg F1)).
+        * eapply add_in_branch_get; eauto.
+        * eapply is_satisfiable_is_satisfiable_add_in_branch; eauto.
+          intros M sigma hinterp hF1. apply hinterp. now left.
+        * now apply branch_contains_add.
+        * intros M sigma hinterp hF2. apply hinterp. now right.
+
+      (* Case: [Or F1 F2] *)
+      + apply is_satisfiable_is_satisfiable_or; auto.
+
+      (* Case: [All F] *)
+      + eapply is_satisfiable_is_satisfiable_add_in_branch; eauto.
+        apply instantiate_imply_all. unfold isLocallyClosed; now cbn.
+
+      (* Case: [Neg (All F)] *)
+      + destruct IHj as (M & hsat0).
+
+        (* TODO: define [M'].
+                 We can arbitrarily pick the values of the arguments of [t] *)
+  Admitted.
+
+  (** An [ExpansionSequence] that has a [closed] [ExpansionTableau] as its last element
+      is actually a tableau proof. *)
+  Lemma hasTableau_iff_ExpansionSequence :
+    forall (Gamma : Con),
+      (exists (sigma : Substitution var Term), hasTableau sko Gamma sigma) <->
+        (exists (seq : ExpansionSequence),
+            hd_error seq = Some (mkExpansionTableau Gamma) /\
+              is_closed_ExpansionTableau (List.last seq (mkExpansionTableau Gamma))).
+  Proof.
+    intro Gamma; split.
+    - intros (sigma & htab); induction htab.
+      + (* exists [mkExpansionTableau Gamma]. *)
+    Admitted.
+End TableauxExpansion.
+
 Section TableauxSoundness.
   Context `{set_nat : set nat} {pred func var : Atom} (sko : Skolemization_ pred func var).
 
@@ -295,68 +528,94 @@ Section TableauxSoundness.
   Let Form := Form_ pred func var.
   Let Term := Term_ func var.
 
+  Definition is_canonical (M : Model pred func) (mu : env M var) (F : Form) :=
+    forall (t : Term) (Gamma : Con) (symbs : sko_record sko),
+      sko t (Neg (All F)) symbs Gamma = true ->
+      (forall (mu : env M var), [[ M # [] # mu '|= Neg (All F) ]]) ->
+      [[ M # [] # mu '|= F {0 \to t} ]].
+
+  Definition super_model :
+    forall (M : Model pred func),
+    exists (M' : Model pred func),
+    forall (F : Form) (mu : env M' var),
+      ((forall (mu0 : env M var), [[ M # [] # mu0 '|= F]]) -> [[ M' # [] # mu '|= F ]]) /\
+        is_canonical M' mu F.
+  Proof.
+    intro M. apply upper_bound_choice with (x := M).
+    intros F hncan. apply NNPP => save.
+    apply hncan; clear hncan. intros mu0; split.
+    + now intro.
+    + intros ??? hsko hdelta. exfalso; apply save; clear save.
+      Admitted.
+
   (** We start by showing that if the root formula of a tableau is satisfiable, then this
       tableau is also satisfiable.
 
       Note that [Gamma] must be a closed context. *)
   Lemma hasTableau_satisfiable :
-    forall {Gamma : Con} {symbs : sko_record sko}
-      {sigma : Substitution var Term} (T : hasTableau_ sko Gamma symbs sigma),
-      (exists (M : Model pred func), forall (mu : env M var),
-          [[ M # [] # mu '|= ctx_to_form Gamma ]]) ->
+    forall {Gamma : Con} {sigma : Substitution var Term} (T : hasTableau sko Gamma sigma)
+      (M : Model pred func),
+      (forall  (mu : env M var), [[ M # [] # mu '|= ctx_to_form Gamma ]]) ->
       exists (M' : Model pred func), forall (mu' : env M' var),
         is_tableau_satisfiable M' mu' T.
   Proof using Type.
-    intros ???? (M & hinterp).
+    intros ???? hinterp.
 
-    (* We start by building the model *)
-    have h :
-      exists (M' : Model pred func),
-        forall (mu' : env M' var), exists (mu : env M var),
-        [[ M' # [] # mu' '|= ctx_to_form Gamma ]] /\
-          (forall (F : Form), [[ M # [] # mu '|= F ]] -> [[ M' # [] # mu' '|= F ]]) /\
-          (forall (F : Form), [[ M' # [] # mu' '|= Neg (All F)  ]] -> [[ M # [] # mu '|= Neg (All F) ]]) /\
-          (M <> M' ->
-           forall (Gamma : Con) (symbs : sko_record sko) (t : Term) (F : Form) (c : M),
-             sko t (Neg (All F)) symbs Gamma = true ->
-             [[  M # [c] # mu '|= Neg F ]] -> [[ M' # [] # mu' '|= Neg F {0 \to t} ]]).
-    { destruct T.
-      1-6: exists M; intro mu; exists mu; repeat split; auto; now intro.
-      have h : forall (mu : env M var), exists (c : M), [[ M # [c] # mu '|= Neg F ]].
-      { intro; specialize (hinterp mu).
-        have hnF := in_form_list_interp H hinterp. apply NNPP => save; apply hnF.
-        intros c; apply NNPP => hG. apply save; now exists c. }
-      admit. }
-    apply NNPP => save; apply save; exists M; intro mu; exfalso; apply save; clear save.
+    have htab : exists (sigma : Substitution var Term), hasTableau sko Gamma sigma by exists sigma.
+    rewrite hasTableau_iff_ExpansionSequence in htab.
+    destruct htab as (seq & e & _).
 
-    destruct h as (M' & hM'). exists M'; intro mu'.
-    specialize (hM' mu'); destruct hM' as (mu & hG' & f & f' & hM'); clear hinterp; induction T.
+    (* We then proceed by induction. *)
+    (* induction T. *)
+    (* - exists M; intro mu; exfalso. have contra := in_form_list_interp i (hinterp mu). *)
+    (*   now cbn in contra. *)
+    (* - exists M; intro mu; now apply satisfiable_hasTableauContr. *)
+    (* - destruct IHT as (M' & IHT). *)
+    (*   + intro; eapply extend_with_equiv_form; eauto. apply neg_neg_equiv. *)
+    (*   + exists M'; intro mu; constructor; apply IHT. *)
+    (* - destruct IHT as (M' & IHT). *)
+    (*   + intro; apply interp_list_commute; eapply extend_with_equiv_form; eauto; apply neg_equiv; *)
+    (*       etransitivity; [apply or_comm|apply or_equiv; symmetry; apply neg_neg_equiv]. *)
+    (*   + exists M'; intro mu; constructor; apply IHT. *)
+        
 
-    - exfalso. have contra := in_form_list_interp i hG'.
-      now cbn in contra.
-    - now apply satisfiable_hasTableauContr.
-    - constructor; apply IHT; auto;
-        eapply extend_with_equiv_form; eauto; apply neg_neg_equiv.
-    - constructor; apply IHT; auto;
-      apply interp_list_commute; eapply extend_with_equiv_form; eauto; apply neg_equiv;
-        etransitivity; [apply or_comm|apply or_equiv; symmetry; apply neg_neg_equiv].
-    - have hinterp' := in_form_list_interp i hG'.
-      destruct hinterp'.
-      + apply satisfiable_hasTableauOr1. apply IHT1; auto.
-        cbn. intros [hnF1 | hnG]; auto.
-      + apply satisfiable_hasTableauOr2. apply IHT2; auto.
-        cbn. intros [hnF2 | hnG]; auto.
-    - constructor. apply IHT; auto.
-      eapply extend_with_imply_form; eauto.
-      apply instantiate_imply_all. now cbn.
-    - constructor. apply IHT; auto.
-      have hdelta := in_form_list_interp i hG'.
-      apply f' in hdelta. cbn in hdelta; apply NNPP => hsave.
-      apply hdelta; intro c; apply NNPP => hnF.
-      set G := Neg F. have hG : interpret_form_ M [c] mu G by apply hnF.
-      cbn in hsave; apply NNPP in hsave; destruct hsave; auto. apply H.
-      change [[ M' # [] # mu' '|= G {0 \to t} ]]. eapply hM'; eauto.
-   Admitted.
+    (*     constructor; apply IHT. *)
+    (*   + apply interp_list_commute; eapply extend_with_equiv_form; eauto; apply neg_equiv; *)
+    (*       etransitivity; [apply or_comm|apply or_equiv; symmetry; apply neg_neg_equiv]. *)
+    (*   + intros G hrank; apply hcan. transitivity (con_rank (Gamma ,, Neg F1 ,, Neg F2)); auto; *)
+    (*                                 transitivity (con_rank (Gamma ,, Neg F1)). *)
+    (*     * apply con_rank_extend with (G := (Neg (Or F1 F2))). *)
+    (*       -- now right. *)
+    (*       -- cbn; lia. *)
+    (*     * apply con_rank_extend with (G := (Neg (Or F1 F2))); auto. *)
+    (*       cbn; lia. *)
+    (*  - have hinterp' := in_form_list_interp i hinterp; destruct hinterp'. *)
+    (*   + apply satisfiable_hasTableauOr1. apply IHT1; auto. *)
+    (*     * intros [hnF1 | hnG]; auto. *)
+    (*     * intros G hrank; apply hcan. *)
+    (*       transitivity (con_rank (Gamma ,, F1)); auto; *)
+    (*         eapply con_rank_extend; eauto; cbn; lia. *)
+    (*   + apply satisfiable_hasTableauOr2. apply IHT2; auto. *)
+    (*     * intros [hnF2 | hnG]; auto. *)
+    (*     * intros G hrank; apply hcan. *)
+    (*       transitivity (con_rank (Gamma ,, F2)); auto; *)
+    (*         eapply con_rank_extend; eauto; cbn; lia. *)
+    (* - constructor; apply IHT; auto. *)
+    (*   + eapply extend_with_imply_form; eauto. *)
+    (*     apply instantiate_imply_all. now cbn. *)
+    (*   + intros G hrank; apply hcan. transitivity (con_rank (Gamma ,, F {0 \to Free x})); auto. *)
+    (*     eapply con_rank_extend; eauto; cbn. rewrite rank_of_opening; lia. *)
+    (* - constructor; apply IHT; auto. *)
+    (*   + have hdelta := in_form_list_interp i hinterp. *)
+    (*     intros [hnG | contra]; auto. apply hnG. *)
+    (*     change [[ M' # [] # mu '|= Neg F {0 \to t} ]]. *)
+    (*     have hrankF : rank F <= con_rank Gamma. *)
+    (*     { transitivity (rank (Neg (All F))); [cbn; lia|]. *)
+    (*       apply con_rank_in; auto. } *)
+    (*     specialize (hcan F hrankF). eapply hcan; eauto. *)
+    (*   + intros G hrank; apply hcan. transitivity (con_rank (Gamma ,, Neg F {0 \to t})); auto. *)
+    (*     eapply con_rank_extend; eauto; cbn. rewrite rank_of_opening; lia. *)
+  Admitted.
 
   (** Of course, no tableau is satisfiable. We start by showing 2 small lemmas: *)
   Lemma in_ctx_in_substituted_ctx :
@@ -402,9 +661,9 @@ Section TableauxSoundness.
   Proof using Type.
     intros ??? hclosedGamma htab.
     rewrite models_iff. intros M. left. intro hsat.
-    have hsat' : exists (M : Model pred func), forall (mu : env M var),
+    have hsat' : forall (mu : env M var),
         interpret_form_ M [] mu (ls_to_form (Neg F :: Gamma)).
-    { exists M; intro mu; change [[ M # [] # mu '|= ls_to_form (Neg F :: Gamma) ]].
+    { intro mu; change [[ M # [] # mu '|= ls_to_form (Neg F :: Gamma) ]].
       rewrite (isClosed_interp_form_env_eq _ _ _ _ (empty_env M var)); auto.
       rewrite isClosedList_isClosedFormList //. }
     eapply hasTableau_satisfiable with (T := htab) in hsat'.
